Refactoring of AuxRel.v and Consistency.v

src/AuxRel.v
@@ -45,11 +45,12 @@ Notation "'Loc_' l" := (fun x => loc x = Some l) (at level 1).
 
 Definition ppo_alt := (sb ∩ same_loc ∪ bob)⁺.
 Definition hb_alt := (ppo_alt ∪ rf)⁺.
-Definition rpo :=
-  (⦗R ∩₁ is_rlx⦘ ⨾ sb ⨾ ⦗F ∩₁ is_acq⦘ ∪
+Definition rpo_imm :=
+  ⦗R ∩₁ is_rlx⦘ ⨾ sb ⨾ ⦗F ∩₁ is_acq⦘ ∪
   ⦗is_acq⦘ ⨾ sb ∪
   sb ⨾ ⦗is_rel⦘ ∪
-  ⦗F ∩₁ is_rel⦘ ⨾ sb ⨾ ⦗W ∩₁ is_rlx⦘)⁺.
+  ⦗F ∩₁ is_rel⦘ ⨾ sb ⨾ ⦗W ∩₁ is_rlx⦘.
+Definition rpo := rpo_imm⁺.
 Definition rhb := (sb ∩ same_loc ∪ rpo ∪ sw)⁺.
 Definition vf := ⦗E⦘ ⨾ ⦗W⦘ ⨾ rf^? ⨾ hb^?.
 Definition srf := (vf ∩ same_loc) ⨾ ⦗R⦘ \ (co ⨾ vf).
@@ -78,13 +79,16 @@ Proof.
   basic_solver.
 Qed.
 
+Lemma rpo_imm_in_sb : rpo_imm ⊆ sb.
+Proof using.
+  unfold rpo_imm.
+  basic_solver.
+Qed.
+
 Lemma rpo_in_sb : rpo ⊆ sb.
 Proof using.
-  unfold rpo. assert (SBTR : sb ≡ sb⁺).
-  { assert (SBTR' : transitive sb) by apply sb_trans. 
-    split; [basic_solver |]. intros x y H. induction H; eauto. }
-  rewrite SBTR at 5. apply clos_trans_mori.
-  unfolder. ins. desf.
+  unfold rpo. rewrite rpo_imm_in_sb.
+  apply ct_of_trans. apply sb_trans.
 Qed.
 
 Lemma wf_rpoE
@@ -137,20 +141,13 @@ Proof using.
   unfolder in SRF; desf.
 Qed.
 
-Lemma wf_same_locE 
-    (WF : Wf G) :
-  same_loc ≡ ⦗E⦘ ⨾ same_loc ⨾ ⦗E⦘.
-Proof using.
-  admit.
-Admitted. 
-
 Lemma wf_rhbE
     (WF : Wf G) :
   rhb ≡ ⦗E⦘ ⨾ rhb ⨾ ⦗E⦘.
 Proof using.
-  unfold rhb. rewrite wf_swE, wf_rpoE, wf_sbE, wf_same_locE; auto.
-  assert (SB_SAMELOC : (⦗E⦘ ⨾ sb ⨾ ⦗E⦘) ∩ (⦗E⦘ ⨾ same_loc ⨾ ⦗E⦘) ≡ (⦗E⦘ ⨾ sb ∩ same_loc ⨾ ⦗E⦘)).
-  { basic_solver. }
+  unfold rhb. rewrite wf_swE, wf_rpoE, wf_sbE; auto.
+  assert (SB_SAMELOC : (⦗E⦘ ⨾ sb ⨾ ⦗E⦘) ∩ same_loc ≡ ⦗E⦘ ⨾ sb ∩ same_loc ⨾ ⦗E⦘).
+  { basic_solver 10. }
   rewrite SB_SAMELOC.
   rewrite <- !seq_union_r, <- !seq_union_l.
   seq_rewrite <- ct_seq_eqv_l. rewrite <- seqA.
